src/proof/simple/list.v
@@ -16,13 +16,13 @@ Lemma wp_State__objListLocked_pod γ l phys_state_l phys_state abs_state kind na
       "Hown_abs" ∷ map_ctx γ.(γ_state) 1 abs_state ∗
       "Hphys_abs_rep" ∷ state_rep phys_state abs_state ∗
       "Hghostpods" ∷ ([∗ map] key ↦ pod ∈ pure_pod_map, key [[ γ.(γ_state) ]]↦ KObjectV.Pod pod) ∗
-      "%Habs_state_well_formed" ∷ ⌜ ∀ k obj, abs_state !! k = Some obj → k = KObjectV.key obj ∧ KObjectV.well_formed obj ⌝
+      "%Habs_state_valid" ∷ ⌜ ∀ k obj, abs_state !! k = Some obj → k = KObjectV.key obj ∧ KObjectV.valid obj ⌝
   }}}
     l @ (ptrT.id apimodel.State.id) @ "objListLocked" #kind #namespace
   {{{ sl ptr_list pure_pod_list, RET #sl;
       sl ↦* map (λ ptr, interface.mk (ptrT.id v1.Pod.id) #ptr) ptr_list ∗
-      ([∗ list] ptr;pure_pod ∈ ptr_list;pure_pod_list, ∃ pod, PodV.deepown_l ptr pod pure_pod 1) ∗
-      ⌜ ∀ p, p ∈ pure_pod_list → PodV.well_formed p ⌝ ∗
+      ([∗ list] ptr;pure_pod ∈ ptr_list;pure_pod_list, PodV.deepown_l ptr pure_pod 1) ∗
+      ⌜ ∀ p, p ∈ pure_pod_list → PodV.valid p ⌝ ∗
       ⌜ ∀ p, p ∈ pure_pod_list → abs_state !! PodV.key p = Some (KObjectV.Pod p) ⌝ ∗
       ⌜ ∀ i j p1 p2, i ≠ j → pure_pod_list !! i = Some p1 → pure_pod_list !! j = Some p2 → PodV.key p1 ≠ PodV.key p2 ⌝ ∗
       ⌜ ∀ p, p ∈ pure_pod_list → v1.namespace_matches namespace p.(PodV.ObjectMeta').(ObjectMetaV.Namespace') ⌝ ∗
